WIP trace proofs

aneris/examples/transactional_consistency/read_uncommitted/trace/implication_trace.v
@@ -18,74 +18,113 @@ Section trace_proof.
 
   (** Ghost theory for wrapped resources *)
 
-  Definition OwnLinTrace (γ : gname) (l : list val) : iProp Σ := True.
+  (* For the OwnLinTrace/OwnLinHist resources and 
+     rules we are reusing trace infrastructure *)
 
-  Definition OwnLinHist (γ : gname) (l : list val) : iProp Σ := True.
+  Definition OwnLinHist (γ : gname) (l : list val) : iProp Σ :=
+    own γ (◯ (gmap_of_trace 0 l)).
 
-  Lemma own_lin_hist (γ : gname) (l h : list val) :
-    OwnLinTrace γ l ==∗ OwnLinTrace γ l ∗ OwnLinHist γ h.
+  Definition OwnLinTrace (γ : gname) (l : list val) : iProp Σ := 
+    own γ (● gmap_of_trace 0 l) ∗ OwnLinHist γ l.
+
+  Lemma own_lin_hist (γ : gname) (l : list val) :
+    OwnLinTrace γ l ==∗ OwnLinTrace γ l ∗ OwnLinHist γ l.
   Proof.
-  Admitted.
+    rewrite /OwnLinTrace.
+    iIntros "(H1 & #H2)".
+    iModIntro.
+    iFrame "#∗".
+  Qed.
 
   Lemma own_lin_prefix (γ : gname) (l h : list val) :
-    OwnLinTrace γ l -∗ 
-    OwnLinHist γ h -∗
-    (OwnLinTrace γ l ∗ OwnLinHist γ h ∗ ⌜h `prefix_of` l⌝).
+    OwnLinTrace γ l ∗ OwnLinHist γ h -∗
+    OwnLinTrace γ l ∗ OwnLinHist γ h ∗ ⌜h `prefix_of` l⌝.
   Proof.
-  Admitted.
+    rewrite /OwnLinTrace /OwnLinHist.
+    iIntros "((H1 & H2) & H3)".
+    iDestruct (own_op with "[$H1 $H3]") as "H".
+    iDestruct (own_valid with "H") as %[Hsub Hvalid]%auth_both_valid_discrete.
+    iDestruct "H" as "(H1 & H3)".
+    iFrame.
+    iPureIntro. 
+    eapply gmap_of_trace_hist_valid_prefix; eauto.
+  Qed.
 
-  Definition OwnTok (γ : gname) : iProp Σ := own γ (Excl ()).
-
-  Lemma own_tok_excl (γ : gname) : 
-    OwnTok γ -∗ OwnTok γ -∗ False.
-  Proof. 
-    iIntros "H1 H2". 
-    by iDestruct (own_valid_2 with "H1 H2") as %?.
+  Lemma own_lin_add (γ : gname) (l: list val) (v : val) :
+    OwnLinTrace γ l ==∗ OwnLinTrace γ (l ++ [v]).
+  Proof.
+    rewrite /OwnLinTrace /OwnLinHist.
+    iIntros "(H1 & H2)".
+    rewrite gmap_of_trace_snoc Nat.add_0_l.
+    iMod (own_update_2 with "H1 H2") as "[H1 H2]".
+    apply auth_update.
+    eapply (alloc_local_update _ _ (length l : nat) (to_agree v)); try done.
+    { 
+      eapply not_elem_of_dom.
+      rewrite gmap_of_trace_dom.
+      intro Hfalse. 
+      lia. 
+    }
+    iModIntro. 
+    iFrame.
   Qed.
 
   (** Predicates for wrapped resources *)
 
-  Definition last_commit : Prop := true.
+  Definition last_commit (c le : val) (ltrace : list val ) : Prop := true.
 
-  Definition open_start : Prop := true. 
+  Definition open_start (c le : val) (ltrace : list val ) : Prop := true. 
 
-  Definition latest_write : Prop := true. 
+  Definition latest_write (c : val) (k : Key) (ov : option val): Prop := true. 
 
-  (** Wrapped resources  *)
-  (* Global Program Instance wrapped_resources (γm1 γm2 γl : gname) `(res : !RU_resources Mdl Σ) : RU_resources Mdl Σ :=
+  Definition tag_eq (e1 e2 : val) : Prop := true.
+
+  (** Extended global invaraint *)
+
+  Definition GlobalInvExt (γm1 γm2 γmk γl : gname) : iProp Σ := 
+    ∃ t lt T, trace_is t ∗ OwnLinTrace γl lt ∗ ⌜lin_trace_of lt t⌝ ∗ ⌜extraction_of lt T⌝ ∗
+      (∃ (m1 : gmap socket_address (local_state * option val)), ghost_map_auth γm1 (1%Qp) m1 ∗ 
+        ((∀ sa s, ⌜m1 !! sa = None ∨ m1 !! sa = Some (s, None)⌝ → ghost_map_auth γmk (1%Qp) ∅) ∨
+          (∀ sa s c, ⌜m1 !! sa = Some (s, Some c)⌝ → 
+            ∃ (mk : gmap (val * Key) (option val)), ghost_map_auth γmk (1%Qp) mk ∗
+            (((⌜s = CanStart⌝ ∗ (∃ e, ⌜last_commit c e lt⌝) ∗ 
+              (∀ k, ⌜k ∈ KVS_keys⌝ → ∃ ov, ghost_map_elem γmk (c, k) (DfracOwn 1%Qp) ov)) ∨ 
+              (∃ domain, ⌜s = Active domain⌝ ∗ (∃ e, ⌜open_start c e lt⌝) ∗
+              (∀ k, ⌜k ∈ KVS_keys ∖ domain⌝ → ∃ ov, ghost_map_elem γmk (c, k) (DfracOwn 1%Qp) ov) ∗
+              (∀ k, ⌜k ∈ domain⌝ → ∀ ov, ⌜mk !! (c, k) = Some ov⌝ → ⌜latest_write c k ov⌝ ))))))) ∗
+      (∃ (m2 : gmap string bool), ⌜∀ (x : string), x ∈ (dom m2) ↔ x ∈ tags t⌝ ∗ ghost_map_auth γm2 (1%Qp) m2 ∗
+        (∀ e_pre tag, ⌜e_pre ∈ t⌝ → ⌜is_pre_event e_pre⌝ → ⌜tagOfEvent e_pre = Some tag⌝ →
+          (∃ e_lin, ⌜e_lin ∈ lt⌝ ∧ ⌜tag_eq e_pre e_lin⌝) → 
+          ghost_map.ghost_map_elem γm2 tag (DfracOwn 1%Qp) true)).
+
+  (** Wrapped resources *)
+  Global Program Instance wrapped_resources (γm1 γm2 γmk γl : gname) `(res : !RU_resources Mdl Σ) : RU_resources Mdl Σ :=
     {|
-      GlobalInv := (GlobalInv ∗ trace_inv trace_inv_name valid_trace_ru ∗ 
-                    ∃ t lt T, trace_is t ∗ OwnLinTrace γl lt ∗ ⌜lin_trace_of lt t⌝ ∗ ⌜extraction_of lin_trace T⌝ ∗
-                      (∃ (m : gmap socket_address local_state), ghost_map_auth γm1 (1%Qp) m ∗ 
-                        (∀ sa s, m !! sa = Some s → 
-                          (((⌜s = CanStart⌝ ∗ (∃ e, ⌜last_commit c e lt⌝) ∗
-                             ∀ k, ⌜k ∈ KVS_keys⌝ → OwnWriteHalf c k ov ∗ OwnWriteHalf c k ov) ∨ 
-                            (⌜s = Active domain⌝ ∗ (∃ e, ⌜open_start c e lt⌝) ∗
-                             (∀ k, ⌜k ∈ domain⌝ → ∃ ov, OwnWriteHalf c k ov ∗ ⌜latest_write c k ov⌝) ∗
-                             (∀ k, ⌜k ∈ KVS_keys / domain⌝ → OwnWriteHalf c k ov ∗ OwnWriteHalf c k ov)))))) ∗
-                      (∃ (m : gmap string gname), ⌜∀ x, x ∈ dom m ↔ x ∈ tags t⌝ ∗ ghost_map_auth γm2 (1%Qp) m ∗
-                        (∀ e_pre tag, ⌜e_pre ∈ t⌝ → ⌜is_pre_event e_pre⌝ → ⌜tagOfEvent e_pre = Some tag⌝ →
-                          (∃ e_lin, ⌜e_lin ∈ lt⌝ ∧ ⌜tag_eq e_pre e_lin⌝) → ∃ γ, m !! tag = Some γ ∗ OwnTok γ)))%I;
-      OwnMemKey k V := (OwnMemKey k V  ∗ (∀ v, ⌜v ∈ V⌝ → ∃ lt tag c, OwnLinHist t ∗ 
-                        ⌜(#(LitString tag), (c, (#"WrLin", (#(LitString k), v))))%V ∈ t⌝))%I;
-      OwnLocalKey k c ov := (OwnLocalKey k c ov ∗ OwnWriteHalf c k ov)%I;
-      ConnectionState c s sa := (ConnectionState c s sa ∗ ghost_map_elem γm1 sa (1%Qp) s)%I; 
+      GlobalInv := (GlobalInv ∗ trace_inv trace_inv_name valid_trace_ru ∗ inv KVS_InvName (GlobalInvExt γm1 γm2 γmk γl))%I;
+      OwnMemKey k V := (OwnMemKey k V  ∗ (∀ v, ⌜v ∈ V⌝ → ∃ lh tag c, OwnLinHist γl lh ∗ 
+                        ⌜(#(LitString tag), (c, (#"WrLin", (#(LitString k), v))))%V ∈ lh⌝))%I;
+      OwnLocalKey k c ov := (OwnLocalKey k c ov ∗ ghost_map_elem γmk (c, k) (DfracOwn 1%Qp) ov ∗ ⌜k ∈ KVS_keys⌝)%I;
+      ConnectionState c sa s := (ConnectionState c sa s ∗ ghost_map_elem γm1 sa (DfracOwn 1%Qp) (s, Some c))%I; 
       IsConnected c sa := IsConnected c sa%I;
       KVS_ru := KVS_ru;
       KVS_Init := KVS_Init%I;
-      KVS_ClientCanConnect sa := KVS_ClientCanConnect sa ∗ ghost_map_elem γm1 sa CanStart%I;
+      KVS_ClientCanConnect sa := (KVS_ClientCanConnect sa ∗ ghost_map_elem γm1 sa (DfracOwn 1%Qp) (CanStart, None))%I;
       Seen k V := Seen k V%I;
     |}.
   Next Obligation.
+    iIntros (????????) "(Hkey & Hghost_elem & %Hin)".
+    iDestruct (res.(read_uncommitted.specs.resources.OwnLocalKey_serializable) with "Hkey") as "(Hkey & Hser)".
+    by iFrame.
+  Qed.
+  Next Obligation.
+    iIntros.
   Admitted.
   Next Obligation.
+    iIntros.
   Admitted.
   Next Obligation.
+    iIntros.
   Admitted.
-  Next Obligation.
-  Admitted.
-  Next Obligation.
-  Admitted. *)
 
   Lemma library_implication `{!anerisG Mdl Σ} (clients : gset socket_address) 
   (lib : KVS_transaction_api) :
